Add more language boilerplate

theories/lang/lang.v
@@ -17,9 +17,21 @@ Module nvm_lang.
 
   Implicit Type ℓ : loc.
 
+  Definition proph_id := positive.
+
   (* Literals of the language. *)
-  Inductive lit : Set :=
-    | LitInt (n : Z) | LitBool (b : bool) | LitUnit | LitLoc ℓ.
+  Inductive literal : Set :=
+    | LitInt (n : Z) | LitBool (b : bool) | LitUnit | LitPoison
+    | LitLoc ℓ | LitProphecy (p: proph_id).
+
+  Inductive un_op : Set := NegOp | MinusUnOp.
+
+  Inductive bin_op : Set :=
+  | PlusOp | MinusOp | MultOp | QuotOp | RemOp (* Arithmetic *)
+  | AndOp | OrOp | XorOp (* Bitwise *)
+  | ShiftLOp | ShiftROp (* Shifts *)
+  | LeOp | LtOp | EqOp (* Relations *)
+  | OffsetOp. (* Pointer offset *)
 
   Inductive expr :=
     (* Embed values inside expressions. *)
@@ -28,18 +40,34 @@ Module nvm_lang.
     | Var (x : string)
     | Rec (f x : binder) (e : expr)
     | App (e1 e2 : expr)
+    (* Base types and their operations *)
+    | UnOp (op : un_op) (e : expr)
+    | BinOp (op : bin_op) (e1 e2 : expr)
+    | If (e0 e1 e2 : expr)
+    (* Products *)
+    | Pair (e1 e2 : expr)
+    | Fst (e : expr)
+    | Snd (e : expr)
+    (* Sums *)
+    | InjL (e : expr)
+    | InjR (e : expr)
+    | Case (e0 : expr) (e1 : expr) (e2 : expr)
     (* Concurrency *)
     | Fork (e : expr)
     (* Memory operations. *)
-    | Read (e : expr)
-    | ReadAcquire (e : expr)
+    | AllocN (e1 e2 : expr)
+    | Load (e : expr)
+    | LoadAcquire (e : expr)
     | Store (e1 e2 : expr)
     | StoreRelease (e1 e2 : expr)
     (* RMW memory operations. *)
     | CmpXchg (e0 : expr) (e1 : expr) (e2 : expr) (* Compare-exchange *)
     | FAA (e1 : expr) (e2 : expr) (* Fetch-and-add *)
+    (* Prophecy *)
+    | NewProph
+    | Resolve (e0 : expr) (e1 : expr) (e2 : expr) (* wrapped expr, proph, val *)
     with val :=
-    | LitV (l : lit)
+    | LitV (l : literal)
     | RecV (f x : binder) (e : expr)
     | PairV (v1 v2 : val)
     | InjLV (v : val)
@@ -48,32 +76,335 @@ Module nvm_lang.
   Bind Scope expr_scope with expr.
   Bind Scope val_scope with val.
 
+  Definition observation : Set := proph_id * (val * val).
+
+  (* Convert values to expressions. *)
   Notation of_val := Val (only parsing).
 
+  (* Convert expressions to values. *)
   Definition to_val (e : expr) : option val :=
     match e with
     | Val v => Some v
     | _ => None
     end.
 
-  (* Evaluation contexts. *)
+  (** Equality and other typeclass stuff *)
+  Lemma to_of_val v : to_val (of_val v) = Some v.
+  Proof. done. Qed.
+
+  Lemma of_to_val e v : to_val e = Some v → of_val v = e.
+  Proof. destruct e=>//=. by intros [= <-]. Qed.
+
+  Global Instance of_val_inj : Inj (=) (=) of_val.
+  Proof. intros. congruence. Qed.
+
+  (* Expressions have decidable equality. *)
+  Global Instance base_lit_eq_dec : EqDecision literal.
+  Proof. solve_decision. Defined.
+  Global Instance un_op_eq_dec : EqDecision un_op.
+  Proof. solve_decision. Defined.
+  Global Instance bin_op_eq_dec : EqDecision bin_op.
+  Proof. solve_decision. Defined.
+  Global Instance expr_eq_dec : EqDecision expr.
+  Proof.
+    refine (
+    fix go (e1 e2 : expr) {struct e1} : Decision (e1 = e2) :=
+      match e1, e2 with
+      | Val v, Val v' => cast_if (decide (v = v'))
+      | Var x, Var x' => cast_if (decide (x = x'))
+      | Rec f x e, Rec f' x' e' =>
+          cast_if_and3 (decide (f = f')) (decide (x = x')) (decide (e = e'))
+      | App e1 e2, App e1' e2' => cast_if_and (decide (e1 = e1')) (decide (e2 = e2'))
+      | UnOp o e, UnOp o' e' => cast_if_and (decide (o = o')) (decide (e = e'))
+      | BinOp o e1 e2, BinOp o' e1' e2' =>
+          cast_if_and3 (decide (o = o')) (decide (e1 = e1')) (decide (e2 = e2'))
+      | If e0 e1 e2, If e0' e1' e2' =>
+          cast_if_and3 (decide (e0 = e0')) (decide (e1 = e1')) (decide (e2 = e2'))
+      | Pair e1 e2, Pair e1' e2' =>
+          cast_if_and (decide (e1 = e1')) (decide (e2 = e2'))
+      | Fst e, Fst e' => cast_if (decide (e = e'))
+      | Snd e, Snd e' => cast_if (decide (e = e'))
+      | InjL e, InjL e' => cast_if (decide (e = e'))
+      | InjR e, InjR e' => cast_if (decide (e = e'))
+      | Case e0 e1 e2, Case e0' e1' e2' =>
+          cast_if_and3 (decide (e0 = e0')) (decide (e1 = e1')) (decide (e2 = e2'))
+      | Fork e, Fork e' => cast_if (decide (e = e'))
+      | AllocN e1 e2, AllocN e1' e2' =>
+          cast_if_and (decide (e1 = e1')) (decide (e2 = e2'))
+      | Load e, Load e' => cast_if (decide (e = e'))
+      | LoadAcquire e, LoadAcquire e' => cast_if (decide (e = e'))
+      | Store e1 e2, Store e1' e2' =>
+          cast_if_and (decide (e1 = e1')) (decide (e2 = e2'))
+      | StoreRelease e1 e2, StoreRelease e1' e2' =>
+          cast_if_and (decide (e1 = e1')) (decide (e2 = e2'))
+      | CmpXchg e0 e1 e2, CmpXchg e0' e1' e2' =>
+          cast_if_and3 (decide (e0 = e0')) (decide (e1 = e1')) (decide (e2 = e2'))
+      | FAA e1 e2, FAA e1' e2' =>
+          cast_if_and (decide (e1 = e1')) (decide (e2 = e2'))
+      | NewProph, NewProph => left _
+      | Resolve e0 e1 e2, Resolve e0' e1' e2' =>
+          cast_if_and3 (decide (e0 = e0')) (decide (e1 = e1')) (decide (e2 = e2'))
+      | _, _ => right _
+      end
+    with gov (v1 v2 : val) {struct v1} : Decision (v1 = v2) :=
+      match v1, v2 with
+      | LitV l, LitV l' => cast_if (decide (l = l'))
+      | RecV f x e, RecV f' x' e' =>
+          cast_if_and3 (decide (f = f')) (decide (x = x')) (decide (e = e'))
+      | PairV e1 e2, PairV e1' e2' =>
+          cast_if_and (decide (e1 = e1')) (decide (e2 = e2'))
+      | InjLV e, InjLV e' => cast_if (decide (e = e'))
+      | InjRV e, InjRV e' => cast_if (decide (e = e'))
+      | _, _ => right _
+      end
+    for go); try (clear go gov; abstract intuition congruence).
+  Defined.
+  Global Instance val_eq_dec : EqDecision val.
+  Proof. solve_decision. Defined.
+
+  (* Expressions are countable. *)
+  Global Instance base_lit_countable : Countable literal.
+  Proof.
+  refine (inj_countable' (λ l, match l with
+    | LitInt n => (inl (inl n), None)
+    | LitBool b => (inl (inr b), None)
+    | LitUnit => (inr (inl false), None)
+    | LitPoison => (inr (inl true), None)
+    | LitLoc l => (inr (inr l), None)
+    | LitProphecy p => (inr (inl false), Some p)
+    end) (λ l, match l with
+    | (inl (inl n), None) => LitInt n
+    | (inl (inr b), None) => LitBool b
+    | (inr (inl false), None) => LitUnit
+    | (inr (inl true), None) => LitPoison
+    | (inr (inr l), None) => LitLoc l
+    | (_, Some p) => LitProphecy p
+    end) _); by intros [].
+  Qed.
+  Global Instance un_op_finite : Countable un_op.
+  Proof.
+  refine (inj_countable' (λ op, match op with NegOp => 0 | MinusUnOp => 1 end)
+    (λ n, match n with 0 => NegOp | _ => MinusUnOp end) _); by intros [].
+  Qed.
+  Global Instance bin_op_countable : Countable bin_op.
+  Proof.
+  refine (inj_countable' (λ op, match op with
+    | PlusOp => 0 | MinusOp => 1 | MultOp => 2 | QuotOp => 3 | RemOp => 4
+    | AndOp => 5 | OrOp => 6 | XorOp => 7 | ShiftLOp => 8 | ShiftROp => 9
+    | LeOp => 10 | LtOp => 11 | EqOp => 12 | OffsetOp => 13
+    end) (λ n, match n with
+    | 0 => PlusOp | 1 => MinusOp | 2 => MultOp | 3 => QuotOp | 4 => RemOp
+    | 5 => AndOp | 6 => OrOp | 7 => XorOp | 8 => ShiftLOp | 9 => ShiftROp
+    | 10 => LeOp | 11 => LtOp | 12 => EqOp | _ => OffsetOp
+    end) _); by intros [].
+  Qed.
+  Global Instance expr_countable : Countable expr.
+  Proof.
+  set (enc :=
+    fix go e :=
+      match e with
+      | Val v => GenNode 0 [gov v]
+      | Var x => GenLeaf (inl (inl x))
+      | Rec f x e => GenNode 1 [GenLeaf (inl (inr f)); GenLeaf (inl (inr x)); go e]
+      | App e1 e2 => GenNode 2 [go e1; go e2]
+      | UnOp op e => GenNode 3 [GenLeaf (inr (inr (inl op))); go e]
+      | BinOp op e1 e2 => GenNode 4 [GenLeaf (inr (inr (inr op))); go e1; go e2]
+      | If e0 e1 e2 => GenNode 5 [go e0; go e1; go e2]
+      | Pair e1 e2 => GenNode 6 [go e1; go e2]
+      | Fst e => GenNode 7 [go e]
+      | Snd e => GenNode 8 [go e]
+      | InjL e => GenNode 9 [go e]
+      | InjR e => GenNode 10 [go e]
+      | Case e0 e1 e2 => GenNode 11 [go e0; go e1; go e2]
+      | Fork e => GenNode 12 [go e]
+      | AllocN e1 e2 => GenNode 13 [go e1; go e2]
+      | Load e => GenNode 15 [go e]
+      | LoadAcquire e => GenNode 21 [go e]
+      | Store e1 e2 => GenNode 16 [go e1; go e2]
+      | StoreRelease e1 e2 => GenNode 22 [go e1; go e2]
+      | CmpXchg e0 e1 e2 => GenNode 17 [go e0; go e1; go e2]
+      | FAA e1 e2 => GenNode 18 [go e1; go e2]
+      | NewProph => GenNode 19 []
+      | Resolve e0 e1 e2 => GenNode 20 [go e0; go e1; go e2]
+      end
+    with gov v :=
+      match v with
+      | LitV l => GenLeaf (inr (inl l))
+      | RecV f x e =>
+          GenNode 0 [GenLeaf (inl (inr f)); GenLeaf (inl (inr x)); go e]
+      | PairV v1 v2 => GenNode 1 [gov v1; gov v2]
+      | InjLV v => GenNode 2 [gov v]
+      | InjRV v => GenNode 3 [gov v]
+      end
+    for go).
+  set (dec :=
+    fix go e :=
+      match e with
+      | GenNode 0 [v] => Val (gov v)
+      | GenLeaf (inl (inl x)) => Var x
+      | GenNode 1 [GenLeaf (inl (inr f)); GenLeaf (inl (inr x)); e] => Rec f x (go e)
+      | GenNode 2 [e1; e2] => App (go e1) (go e2)
+      | GenNode 3 [GenLeaf (inr (inr (inl op))); e] => UnOp op (go e)
+      | GenNode 4 [GenLeaf (inr (inr (inr op))); e1; e2] => BinOp op (go e1) (go e2)
+      | GenNode 5 [e0; e1; e2] => If (go e0) (go e1) (go e2)
+      | GenNode 6 [e1; e2] => Pair (go e1) (go e2)
+      | GenNode 7 [e] => Fst (go e)
+      | GenNode 8 [e] => Snd (go e)
+      | GenNode 9 [e] => InjL (go e)
+      | GenNode 10 [e] => InjR (go e)
+      | GenNode 11 [e0; e1; e2] => Case (go e0) (go e1) (go e2)
+      | GenNode 12 [e] => Fork (go e)
+      | GenNode 13 [e1; e2] => AllocN (go e1) (go e2)
+      | GenNode 15 [e] => Load (go e)
+      | GenNode 21 [e] => LoadAcquire (go e)
+      | GenNode 16 [e1; e2] => Store (go e1) (go e2)
+      | GenNode 22 [e1; e2] => StoreRelease (go e1) (go e2)
+      | GenNode 17 [e0; e1; e2] => CmpXchg (go e0) (go e1) (go e2)
+      | GenNode 18 [e1; e2] => FAA (go e1) (go e2)
+      | GenNode 19 [] => NewProph
+      | GenNode 20 [e0; e1; e2] => Resolve (go e0) (go e1) (go e2)
+      | _ => Val $ LitV LitUnit (* dummy *)
+      end
+    with gov v :=
+      match v with
+      | GenLeaf (inr (inl l)) => LitV l
+      | GenNode 0 [GenLeaf (inl (inr f)); GenLeaf (inl (inr x)); e] => RecV f x (go e)
+      | GenNode 1 [v1; v2] => PairV (gov v1) (gov v2)
+      | GenNode 2 [v] => InjLV (gov v)
+      | GenNode 3 [v] => InjRV (gov v)
+      | _ => LitV LitUnit (* dummy *)
+      end
+    for go).
+  refine (inj_countable' enc dec _).
+  refine (fix go (e : expr) {struct e} := _ with gov (v : val) {struct v} := _ for go).
+  - destruct e as [v| | | | | | | | | | | | | | | | | | | | | |]; simpl; f_equal;
+      [exact (gov v)|done..].
+  - destruct v; by f_equal.
+  Qed.
+  Global Instance val_countable : Countable val.
+  Proof. refine (inj_countable of_val to_val _); auto using to_of_val. Qed.
+
+  (** Evaluation contexts *)
   Inductive ectx_item :=
-  .
+    (* Functions and application. *)
+    | AppLCtx (v2 : val)
+    | AppRCtx (e1 : expr)
+    (* Base types and their operations *)
+    | UnOpCtx (op : un_op)
+    | BinOpLCtx (op : bin_op) (v2 : val)
+    | BinOpRCtx (op : bin_op) (e1 : expr)
+    | IfCtx (e1 e2 : expr)
+    (* Products *)
+    | PairLCtx (v2 : val)
+    | PairRCtx (e1 : expr)
+    | FstCtx
+    | SndCtx
+    (* Sums *)
+    | InjLCtx
+    | InjRCtx
+    | CaseCtx (e1 : expr) (e2 : expr)
+    (* Memory operations. *)
+    | AllocNLCtx (v2 : val)
+    | AllocNRCtx (e1 : expr)
+    | LoadCtx
+    | LoadAcquireCtx
+    | StoreLCtx (v2 : val)
+    | StoreRCtx (e1 : expr)
+    | StoreReleaseLCtx (v2 : val)
+    | StoreReleaseRCtx (e1 : expr)
+    (* RMW memory operations. *)
+    | CmpXchgLCtx (v1 : val) (v2 : val)
+    | CmpXchgMCtx (e0 : expr) (v2 : val)
+    | CmpXchgRCtx (e0 : expr) (e1 : expr)
+    | FaaLCtx (v2 : val)
+    | FaaRCtx (e1 : expr).
 
-  (* [fill_item] inserts an expression into an evaluation context. On paper this
-  is often denoted K[e]. *)
-  Fixpoint fill_item (Ki : ectx_item) (e : expr) : expr :=
-    e.
+  (* [fill_item] inserts an expression into an evaluation context item. *)
+  Definition fill_item (Ki : ectx_item) (e : expr) : expr :=
+    match Ki with
+    | AppLCtx v2 => App e (of_val v2)
+    | AppRCtx e1 => App e1 e
+    | UnOpCtx op => UnOp op e
+    | BinOpLCtx op v2 => BinOp op e (Val v2)
+    | BinOpRCtx op e1 => BinOp op e1 e
+    | IfCtx e1 e2 => If e e1 e2
+    | PairLCtx v2 => Pair e (Val v2)
+    | PairRCtx e1 => Pair e1 e
+    | FstCtx => Fst e
+    | SndCtx => Snd e
+    | InjLCtx => InjL e
+    | InjRCtx => InjR e
+    | CaseCtx e1 e2 => Case e e1 e2
+    | AllocNLCtx v2 => AllocN e (Val v2)
+    | AllocNRCtx e1 => AllocN e1 e
+    | LoadCtx => Load e
+    | LoadAcquireCtx => Load e
+    | StoreLCtx v2 => Store e (Val v2)
+    | StoreRCtx e1 => Store e1 e
+    | StoreReleaseLCtx v2 => Store e (Val v2)
+    | StoreReleaseRCtx e1 => Store e1 e
+    | CmpXchgLCtx v1 v2 => CmpXchg e (Val v1) (Val v2)
+    | CmpXchgMCtx e0 v2 => CmpXchg e0 e (Val v2)
+    | CmpXchgRCtx e0 e1 => CmpXchg e0 e1 e
+    | FaaLCtx v2 => FAA e (Val v2)
+    | FaaRCtx e1 => FAA e1 e
+    end.
 
-  (** Substitution *)
-  (* Replace occurrences of [x] in [e] with [v]. *)
-  Fixpoint subst (x : string) (v : val) (e : expr)  : expr := e.
+  (** Substitution, replaces occurrences of [x] in [e] with [v]. *)
+  Fixpoint subst (x : string) (v : val) (e : expr)  : expr :=
+    match e with
+    | Val _ => e
+    | Var y => if decide (x = y) then Val v else Var y
+    | Rec f y e =>
+      Rec f y $ if decide (BNamed x ≠ f ∧ BNamed x ≠ y) then subst x v e else e
+    | App e1 e2 => App (subst x v e1) (subst x v e2)
+    | UnOp op e => UnOp op (subst x v e)
+    | BinOp op e1 e2 => BinOp op (subst x v e1) (subst x v e2)
+    | If e0 e1 e2 => If (subst x v e0) (subst x v e1) (subst x v e2)
+    | Pair e1 e2 => Pair (subst x v e1) (subst x v e2)
+    | Fst e => Fst (subst x v e)
+    | Snd e => Snd (subst x v e)
+    | InjL e => InjL (subst x v e)
+    | InjR e => InjR (subst x v e)
+    | Case e0 e1 e2 => Case (subst x v e0) (subst x v e1) (subst x v e2)
+    | Fork e => Fork (subst x v e)
+    | AllocN e1 e2 => AllocN (subst x v e1) (subst x v e2)
+    | Load e => Load (subst x v e)
+    | LoadAcquire e => LoadAcquire (subst x v e)
+    | Store e1 e2 => Store (subst x v e1) (subst x v e2)
+    | StoreRelease e1 e2 => StoreRelease (subst x v e1) (subst x v e2)
+    | CmpXchg e0 e1 e2 => CmpXchg (subst x v e0) (subst x v e1) (subst x v e2)
+    | FAA e1 e2 => FAA (subst x v e1) (subst x v e2)
+    | NewProph => NewProph
+    | Resolve ex e1 e2 => Resolve (subst x v ex) (subst x v e1) (subst x v e2)
+    end.
 
+  Definition subst' (mx : binder) (v : val) : expr → expr :=
+    match mx with BNamed x => subst x v | BAnon => id end.
+
+  Definition un_op_eval (op : un_op) (v : val) : option val :=
+    match op, v with
+    | NegOp, LitV (LitBool b) => Some $ LitV $ LitBool (negb b)
+    (* | NegOp, LitV (LitInt n) => Some $ LitV $ LitInt (Z.lnot n) *) (* Negation on ints, let's leave that out for now. *)
+    | MinusUnOp, LitV (LitInt n) => Some $ LitV $ LitInt (- n)
+    | _, _ => None
+    end.
+
+  Definition bin_op_eval (op: bin_op) (v1 v2: val) : option val :=
+    match op with
+    | PlusOp => match v1, v2 with
+                | LitV (LitInt n1), LitV (LitInt n2) =>
+                  Some (LitV (LitInt (n1 + n2)))
+                | _, _ => None
+                end
+    | EqOp => Some (LitV $ LitBool $ bool_decide (v1 = v2))
+    | PairOp => Some (PairV v1 v2)
+    end.
 
   (* Per thread expression reductions. Note: This does not fit the format that
   Iris expects---we mold it later on. *)
-  Inductive head_step : expr → option mem_event → expr → list expr → Prop :=
+  (* Inductive head_step : expr → option mem_event → expr → list expr → Prop := *)
 
-  Inductive head_step : expr → state → list observation → expr → state → list expr → Prop :=
+  (* Inductive head_step : expr → state → list observation → expr → state → list expr → Prop := *)
 
 End nvm_lang.
